library/init/data/option/basic.lean
@@ -84,4 +84,4 @@ instance {α : Type u} [DecidableEq α] : DecidableEq (Option α) :=
    | (isTrue e)  := isTrue (congrArg (@some α) e)
    | (isFalse n) := isFalse (λ h, Option.noConfusion h (λ e, absurd e n))}
 
-instance {α : Type u} [HasLt α] : HasLt (Option α) := ⟨Option.lt (<)⟩
+instance {α : Type u} [HasLess α] : HasLess (Option α) := ⟨Option.lt (<)⟩
